seiostar/ExamplesIORefinements.fst
@@ -1,0 +1,38 @@
+module ExamplesIORefinements
+
+open FStar.Tactics
+open IOStar
+
+
+let simple_erase_ref (x:bool{x == true}) : io (bool) =
+  return x
+
+let simple_ref_id (x:bool{x == true}) : io (x:bool{x == true}) =
+  return x
+
+let simple_reref_id (x:bool{x == true}) : io (x:bool{x == true \/ x == false}) =
+  return x
+
+let simple_ref_bind (x:bool{x == true}) : io (y:bool{y == true \/ y == false})
+  by (dump "H") =
+  let!@ _ = io_call OOpen "./string" in
+  // F* does not support nested subtyping and if return infers the type 
+  // from the argument instead of the return type, we need to annotate
+  return #(y:bool{y == true \/ y == false}) x
+
+let simple_ref_bind2 () : io (resexn nat) =
+  let!@ fd = io_call OOpen "./string" in
+  return #(resexn nat) (
+    match fd with
+    | Inl fd -> 
+      if fd >= 0 
+      then Inl fd
+      else Inr ()
+    | Inr _ -> Inr ())
+
+[@expect_failure]
+let connect_refs_to_specs () : io (resexn nat) by (dump "H") =
+  let!@ fd : resexn file_descr = io_call OOpen "./string" in
+  match fd with
+  | Inl fd -> return (Inl (fd <: nat)) // CA: to prove this, one needs to use the postcondition of OOpen, which is not available
+  | Inr _ -> return (Inr ())
